theories/ghost_state.v
@@ -1,0 +1,97 @@
+From stdpp Require Import coPset.
+From Coq Require Import QArith Qcanon.
+From iris.algebra Require Import big_op gmap frac agree.
+From iris.algebra Require Import csum excl auth cmra_big_op numbers.
+From iris.bi Require Import fractional.
+From iris.base_logic Require Export lib.own.
+From iris.base_logic.lib Require Import ghost_map.
+From iris.proofmode Require Export tactics.
+From isla Require Export opsem.
+Set Default Proof Using "Type".
+Import uPred.
+
+Class heapG Σ := HeapG {
+  heap_instrs_inG :> ghost_mapG Σ addr (list trc);
+  heap_instrs_name : gname;
+  heap_regs_inG :> ghost_mapG Σ string valu;
+}.
+
+Class threadG := ThreadG {
+  thread_regs_name : gname;
+}.
+
+Section definitions.
+  Context `{!heapG Σ}.
+
+  Definition instr_def (a : addr) (i: list trc) : iProp Σ :=
+    a ↪[ heap_instrs_name ]□ i.
+  Definition instr_aux : seal (@instr_def). by eexists. Qed.
+  Definition instr := unseal instr_aux.
+  Definition instr_eq : @instr = @instr_def :=
+    seal_eq instr_aux.
+
+  Definition instr_ctx (intrs : gmap addr (list trc)) : iProp Σ :=
+    ghost_map_auth heap_instrs_name 1 intrs.
+
+  Definition reg_mapsto_def (γ : gname) (r : string) (q : frac) (v: valu) : iProp Σ :=
+    r ↪[ γ ]{# q} v.
+  Definition reg_mapsto_aux : seal (@reg_mapsto_def). by eexists. Qed.
+  Definition reg_mapsto := unseal reg_mapsto_aux.
+  Definition reg_mapsto_eq : @reg_mapsto = @reg_mapsto_def :=
+    seal_eq reg_mapsto_aux.
+
+  Definition regs_ctx `{!threadG} (regs : reg_map) : iProp Σ :=
+    ghost_map_auth thread_regs_name 1 (reg_map_to_gmap regs).
+
+  Definition state_ctx (σ : seq_global_state) (κs : list seq_label) : iProp Σ :=
+    ⌜True⌝ ∗
+    instr_ctx σ.(seq_instrs).
+
+  Definition thread_ctx `{!threadG} (regs : reg_map) : iProp Σ :=
+    regs_ctx regs.
+
+End definitions.
+
+Notation "r ↦ᵣ{ q } v" := (reg_mapsto thread_regs_name r q v)
+  (at level 20, q at level 50, format "r  ↦ᵣ{ q }  v") : bi_scope.
+Notation "r ↦ᵣ v" := (reg_mapsto thread_regs_name r 1 v) (at level 20) : bi_scope.
+
+Section instr.
+  Context `{!heapG Σ}.
+  Global Instance instr_pers a i : Persistent (instr a i).
+  Proof. rewrite instr_eq. by apply _. Qed.
+
+  Global Instance instr_tl a i : Timeless (instr a i).
+  Proof. rewrite instr_eq. by apply _. Qed.
+
+  Lemma instr_lookup instrs a i :
+    instr_ctx instrs -∗ instr a i -∗ ⌜instrs !! a = Some i⌝.
+  Proof. rewrite instr_eq. by apply ghost_map_lookup. Qed.
+
+End instr.
+
+Section reg.
+  Context `{!heapG Σ}.
+
+  Global Instance reg_mapsto_tl γ r q v : Timeless (reg_mapsto γ r q v).
+  Proof. rewrite reg_mapsto_eq. by apply _. Qed.
+
+  Lemma reg_mapsto_lookup `{!threadG} regs r q v :
+    regs_ctx regs -∗ r ↦ᵣ{q} v -∗ ⌜regs !! r = Some v⌝.
+  Proof.
+    rewrite reg_mapsto_eq.
+    iIntros "Hregs Hreg".
+    iDestruct (ghost_map_lookup with "Hregs Hreg") as %?.
+    by rewrite -reg_map_to_gmap_lookup.
+  Qed.
+
+  Lemma reg_mapsto_update `{!threadG} regs r v v' :
+    regs_ctx regs -∗ r ↦ᵣ v ==∗ regs_ctx (<[r := v']>regs) ∗ r ↦ᵣ v'.
+  Proof.
+    iIntros "Hregs Hreg".
+    iDestruct (reg_mapsto_lookup with "Hregs Hreg") as %?.
+    rewrite reg_mapsto_eq.
+    iMod (ghost_map_update with "Hregs Hreg") as "[? $]".
+    by erewrite reg_map_to_gmap_insert.
+  Qed.
+End reg.
