theories/lifting.v
@@ -1,0 +1,117 @@
+From iris.proofmode Require Import tactics.
+From iris.program_logic Require Export weakestpre.
+From iris.program_logic Require Import ectx_lifting.
+From isla Require Export opsem ghost_state.
+Set Default Proof Using "Type".
+Import uPred.
+
+Class islaG Σ := IslaG {
+  islaG_invG : invG Σ;
+  islaG_gen_heapG :> heapG Σ
+}.
+
+Instance isla_irisG `{!islaG Σ} : irisG isla_lang Σ := {
+  iris_invG := islaG_invG;
+  state_interp σ _ κs _ := state_ctx σ κs;
+  fork_post _ := True%I;
+  num_laters_per_step _ := 0%nat;
+  state_interp_mono _ _ _ _ := fupd_intro _ _;
+}.
+Global Opaque iris_invG.
+
+Instance into_val_val e v `{!TCEq (seq_to_val e) (Some v)} : IntoVal e v.
+Proof. apply of_to_val. by apply TCEq_eq. Qed.
+
+Local Hint Extern 0 (reducible _ _) => eexists _, _, _, _; simpl : core.
+
+
+Definition wp_asm_def `{!islaG Σ} `{!threadG} (e : trc) : iProp Σ :=
+  (∀ θ, ⌜θ.(seq_trace) = e⌝ -∗ ⌜θ.(seq_nb_state) = false⌝ -∗ thread_ctx θ.(seq_regs) -∗
+    WP θ {{ _, True }}).
+Definition wp_asm_aux `{!islaG Σ} `{!threadG} : seal (@wp_asm_def Σ _ _). by eexists. Qed.
+Definition wp_asm `{!islaG Σ} `{!threadG} : trc → iProp Σ := (wp_asm_aux).(unseal).
+Definition wp_asm_eq `{!islaG Σ} `{!threadG} : wp_asm = @wp_asm_def Σ _ _ := (wp_asm_aux).(seal_eq).
+
+Notation WPasm := wp_asm.
+
+Ltac inv_seq_step :=
+  simplify_eq/=;
+  lazymatch goal with
+  | H : seq_step _ _ _ _ _ _ |- _ => inversion H; clear H
+  end;
+  simplify_eq/=;
+  lazymatch goal with
+  | H : trace_step _ _ _ |- _ => inversion H; clear H
+  end;
+  simplify_eq/=;
+  destruct_and?;
+  simplify_eq/=.
+
+
+Section lifting.
+  Context `{!islaG Σ} `{!threadG}.
+
+  Lemma wp_asm_unfold e :
+    WPasm e ⊣⊢ wp_asm_def e.
+  Proof. by rewrite wp_asm_eq. Qed.
+
+  Lemma wp_next_instr nPC bPC_changed a newPC newPC_changed ins :
+    next_pc nPC bPC_changed = Some (a, newPC, newPC_changed) →
+    (∃ i, i ∈ ins) →
+    "_PC" ↦ᵣ Val_Bits nPC -∗
+    "__PC_changed" ↦ᵣ Val_Bool bPC_changed -∗
+    instr a ins -∗
+    (∀ i, ⌜i ∈ ins⌝ -∗ "_PC" ↦ᵣ newPC -∗ "__PC_changed" ↦ᵣ newPC_changed -∗ WPasm i) -∗
+    WPasm [].
+  Proof.
+    iIntros (Hnext [??]) "HPC Hchanged Hi Hcont". setoid_rewrite wp_asm_unfold.
+    iIntros ([???]) "/= -> -> Hθ".
+    iApply wp_lift_step; [done|].
+    iIntros (σ1 ??? ?) "(%&Hictx)".
+    iApply fupd_mask_intro; first set_solver. iIntros "HE".
+    iDestruct (reg_mapsto_lookup with "Hθ HPC") as %HPC.
+    iDestruct (reg_mapsto_lookup with "Hθ Hchanged") as %Hchanged.
+    iDestruct (instr_lookup with "Hictx Hi") as %Hi.
+    iSplit. {
+      iPureIntro. eexists _, _, _, _; simpl. econstructor; [done |by econstructor|]; simpl.
+      eexists _, _. rewrite /next_pc_regs HPC Hchanged. cbn -[next_pc]. rewrite Hnext/=.
+      split_and!; [done| done|]. by rewrite Hi.
+    }
+    iIntros "!>" (????). iMod "HE" as "_". iModIntro.
+    inv_seq_step.
+    revert select (∃ _, _) => -[?[?]].
+    rewrite /next_pc_regs HPC Hchanged. cbn -[next_pc]. rewrite Hnext/= => -[[<- <-] [-> ]].
+    rewrite Hi => -[? ?].
+    iFrame. iSplitL; [|done].
+    iMod (reg_mapsto_update with "Hθ HPC") as "[Hθ HPC]".
+    iMod (reg_mapsto_update with "Hθ Hchanged") as "[Hθ Hchanged]".
+    iApply ("Hcont" with "[//] HPC Hchanged"); [done|done|].
+    iFrame.
+  Qed.
+
+  Lemma wp_read_reg r v v' ann es q:
+    r ↦ᵣ{q} v' -∗
+    (⌜v = v'⌝ -∗ r ↦ᵣ{q} v' -∗ WPasm es) -∗
+    WPasm (ReadReg r [] v ann :: es).
+  Proof.
+    iIntros "Hr Hcont". setoid_rewrite wp_asm_unfold.
+    iIntros ([???]) "/= -> -> Hθ".
+    iApply wp_lift_step; [done|].
+    iIntros (σ1 ??? ?) "(%&Hictx)".
+    iApply fupd_mask_intro; first set_solver. iIntros "HE".
+    iDestruct (reg_mapsto_lookup with "Hθ Hr") as %Hr.
+    move: (Hr) => /reg_map_lookup_is_local ?.
+    iSplit. {
+      iPureIntro. eexists _, _, _, _; simpl. econstructor; [done |by econstructor|]; simpl.
+      case_match; [|done]. by right.
+    }
+    iIntros "!>" (????). iMod "HE" as "_". iModIntro.
+    inv_seq_step. case_match; [ destruct_or!; destruct_and! | done];
+      unfold register_name in *; simplify_eq.
+    all: iFrame; iSplitL; [|done].
+    2: { by iApply wp_value. }
+    iApply ("Hcont" with "[//] Hr"); [done|done|].
+    iFrame.
+  Qed.
+
+End lifting.
